new theorem for code_labels
plan is to both check the ptree and check the result in a single pass
down the code. (both can be computed outside the logic.) the theorem
proved justifies the sufficiency of doing the check.

labels_computeLib not updated.

bootstrap/labels_computeScript.sml
@@ -21,9 +21,36 @@ val inst_labels_fn_def = save_thm("inst_labels_fn_def",
   inst_labels_fn_def |> SIMP_RULE std_ss [LET_DEF]);
 
 val good_label_map_def = Define`
-  (good_label_map [] p l fn ⇔ T) ∧
-  (good_label_map (Label n::xs) p l fn ⇔ fn ' n = SOME p ∧ good_label_map xs p l fn) ∧
-  (good_label_map (x::xs) p l fn = good_label_map xs (p + l x + 1:num) l fn)`
+  (good_label_map [] [] p l pt ⇔ T) ∧
+  (good_label_map [] us p l pt ⇔ F) ∧
+  (good_label_map (Label n::xs) us  p l pt ⇔ pt ' n = SOME p ∧ good_label_map xs us p l pt) ∧
+  (good_label_map (PushPtr (Lab n)::xs) (PushPtr (Addr k)::us) p l pt ⇔
+   pt ' n = SOME k ∧ good_label_map xs us (p + SUC(l (PushPtr (Lab n)))) l pt) ∧
+  (good_label_map (PushPtr (Lab n)::xs) _ p l pt ⇔ F) ∧
+  (good_label_map (Call    (Lab n)::xs) (Call    (Addr k)::us) p l pt ⇔
+   pt ' n = SOME k ∧ good_label_map xs us (p + SUC(l (Call    (Lab n)))) l pt) ∧
+  (good_label_map (Call (Lab n)::xs) _ p l pt ⇔ F) ∧
+  (good_label_map (Jump    (Lab n)::xs) (Jump    (Addr k)::us) p l pt ⇔
+   pt ' n = SOME k ∧ good_label_map xs us (p + SUC(l (Jump    (Lab n)))) l pt) ∧
+  (good_label_map (Jump (Lab n)::xs) _ p l pt ⇔ F) ∧
+  (good_label_map (JumpIf  (Lab n)::xs) (JumpIf  (Addr k)::us) p l pt ⇔
+   pt ' n = SOME k ∧ good_label_map xs us (p + SUC(l (JumpIf  (Lab n)))) l pt) ∧
+  (good_label_map (JumpIf (Lab n)::xs) _ p l pt ⇔ F) ∧
+  (good_label_map (x::xs) (u::us) p l pt ⇔ x = u ∧ good_label_map xs us (p + SUC(l x)) l pt) ∧
+  (good_label_map (x::xs) [] p l pt ⇔ F)`
+
+val good_label_map_clauses = store_thm("good_label_map_clauses",``
+  (good_label_map [] [] p l pt ⇔ T) ∧
+  (good_label_map (Label n        ::xs)                    us  p l pt ⇔ pt ' n = SOME p ∧ good_label_map xs us p l pt) ∧
+  (good_label_map (PushPtr (Lab n)::xs) (PushPtr (Addr k)::us) p l pt ⇔
+   pt ' n = SOME k ∧ good_label_map xs us (p + SUC(l (PushPtr (Lab n)))) l pt) ∧
+  (good_label_map (Call    (Lab n)::xs) (Call    (Addr k)::us) p l pt ⇔
+   pt ' n = SOME k ∧ good_label_map xs us (p + SUC(l (Call    (Lab n)))) l pt) ∧
+  (good_label_map (Jump    (Lab n)::xs) (Jump    (Addr k)::us) p l pt ⇔
+   pt ' n = SOME k ∧ good_label_map xs us (p + SUC(l (Jump    (Lab n)))) l pt) ∧
+  (good_label_map (JumpIf  (Lab n)::xs) (JumpIf  (Addr k)::us) p l pt ⇔
+   pt ' n = SOME k ∧ good_label_map xs us (p + SUC(l (JumpIf  (Lab n)))) l pt)``,
+  simp[good_label_map_def])
 
 val labels_set_def = Define`
   labels_set code = { n | MEM (Label n) code }`
@@ -33,13 +60,38 @@ val FDOM_collect_labels_labels_set = store_thm("FDOM_collect_labels_labels_set",
   gen_tac >> Induct >> simp[collect_labels_def,labels_set_def] >>
   Cases >> simp[labels_set_def] >> simp[pred_setTheory.EXTENSION])
 
+(*
+val good_labels_map_length = store_thm("good_labels_map_length",
+  ``∀ls us p l fn. good_label_map ls us p l fn ⇒ LENGTH us = LENGTH (FILTER ($~ o is_Label) ls)``,
+  Induct >- (
+    simp[good_label_map_def] >>
+    Cases >> simp[good_label_map_def] ) >>
+  Cases >> simp[good_label_map_def] >>
+  Cases >> simp[good_label_map_def] >>
+  rpt strip_tac >> fs[] >> res_tac >> fs[] >>
+  Cases_on`l`>>Cases_on`h`>>fs[good_label_map_def]>>
+  Cases_on`l`>>fs[good_label_map_def]>>
+  res_tac >> fs[])
+*)
+
 val good_label_map_collect_labels = store_thm("good_label_map_collect_labels",
-  ``∀fn l ls p. good_label_map ls p l fn ⇒ ∀x. x ∈ FDOM (collect_labels ls p l) ⇒ FLOOKUP (collect_labels ls p l) x = fn ' x``,
+  ``∀fn l ls us p. good_label_map ls us p l fn ⇒ ∀x. x ∈ FDOM (collect_labels ls p l) ⇒ FLOOKUP (collect_labels ls p l) x = fn ' x``,
   ntac 2 gen_tac >> Induct >>
   simp[collect_labels_def,good_label_map_def] >>
   Cases >> simp[good_label_map_def,collect_labels_def,FLOOKUP_UPDATE] >>
+  Cases >> simp[good_label_map_def] >>
   rw[] >> fs[] >>
-  rw[] >> fs[])
+  rw[] >> fs[] >>
+  TRY (
+    first_x_assum (match_mp_tac o MP_CANON) >>
+    fsrw_tac[ARITH_ss][arithmeticTheory.ADD1] >>
+    metis_tac[] ) >>
+  Cases_on`l'`>>fs[good_label_map_def]>>
+  Cases_on`h`>>fs[good_label_map_def]>>
+  Cases_on`l'`>>fs[good_label_map_def] >> rw[] >>
+  first_x_assum (match_mp_tac o MP_CANON) >>
+  fsrw_tac[ARITH_ss][arithmeticTheory.ADD1] >>
+  metis_tac[] )
 
 val inst_labels_fn_intro0 = prove(
   ``∀f1 f2 ls ls0.
@@ -63,13 +115,53 @@ val inst_labels_fn_intro0 = prove(
       simp[] >> metis_tac[] )))
 
 val inst_labels_fn_intro = store_thm("inst_labels_fn_intro",
-  ``∀fn l ls. good_label_map ls 0 l fn ∧ code_labels_ok ls ⇒
+  ``∀fn l ls us. good_label_map ls us 0 l fn ∧ code_labels_ok ls ⇒
           code_labels l ls = inst_labels_fn fn ls``,
    rw[code_labels_def,all_labels_def] >>
    imp_res_tac good_label_map_collect_labels >> fs[] >>
    match_mp_tac inst_labels_fn_intro0 >>
    qexists_tac`[]` >>
    fs[FDOM_collect_labels_labels_set])
+
+val good_label_map_inst_labels = store_thm("good_label_map_inst_labels",
+  ``∀fn l ls us p ls0. good_label_map ls us p l fn ∧ code_labels_ok (ls0++ls) ⇒
+      inst_labels_fn fn ls = us``,
+  ntac 2 gen_tac >> Induct >>
+  simp[good_label_map_def,inst_labels_fn_def] >- (
+    Cases >> simp[good_label_map_def] ) >>
+  Cases >> simp[good_label_map_def,inst_labels_fn_def] >>
+  Cases >> simp[good_label_map_def] >>
+  rw[] >> fs[] >>
+  rw[] >> fs[] >>
+  simp[inst_labels_def] >>
+  TRY (
+    first_x_assum (match_mp_tac o MP_CANON) >>
+    fsrw_tac[ARITH_ss][arithmeticTheory.ADD1] >>
+    fs[code_labels_ok_def,uses_label_thm] >>
+    HINT_EXISTS_TAC >> simp[] >>
+    TRY(qexists_tac`ls0`>>simp[]>>metis_tac[]) >>
+    qexists_tac`Label n :: ls0` >> simp[] >> metis_tac[]) >>
+  Cases_on`l'`>>fs[good_label_map_def,inst_labels_fn_def]>>
+  TRY (
+    first_x_assum (match_mp_tac o MP_CANON) >>
+    HINT_EXISTS_TAC >> simp[] >>
+    fs[code_labels_ok_def,uses_label_thm] >>
+    metis_tac[] ) >>
+  Cases_on`h`>>fs[good_label_map_def,inst_labels_fn_def]>>
+  Cases_on`l'`>>fs[good_label_map_def,inst_labels_fn_def] >>
+  first_x_assum (match_mp_tac o MP_CANON) >>
+  HINT_EXISTS_TAC >> simp[] >>
+  fs[code_labels_ok_def,uses_label_thm] >>
+  metis_tac[] )
+
+val code_labels_elim = store_thm("code_labels_elim",
+  ``∀fn l ls us .
+      good_label_map ls us 0 l fn ∧ code_labels_ok ls ⇒
+      code_labels l ls = us``,
+  rw[] >>
+  imp_res_tac good_label_map_inst_labels >>
+  pop_assum(qspec_then`[]`mp_tac) >> rw[] >>
+  metis_tac[inst_labels_fn_intro])
 
 val _ = Parse.set_fixity"="(Parse.Infix(Parse.NONASSOC, 100)) (* required to load patriciaLib later *)
 
